<?xml version="1.0" encoding="UTF-8"?>




	  
	  <section xml:id="section-141-GW-4" xmlns:xi="http://www.w3.org/2001/XInclude">
		  <title>
			  Practice Gateway Exam 4
		  </title>
		  
		  <xi:include href="./GW-141-Instructions.ptx" />
		  
		  
		  <exercises>
			  
			  <exercise>
				  <statement>
					  <p>
						  <m>\displaystyle \int (r+1)^3 \, dr </m>
					  </p>

				  </statement>
			  
			  
				  <solution>
					  <p>
						  Use substitution with <m>u=r+1</m> and <m>du=dr</m>:
						  <md>
							  <mrow>
								  \int (r+1)^3 \, dr \amp = \int u^3 \, du
							  </mrow>
							  <mrow>
								  \amp = \frac{u^4}{4}+C
							  </mrow>
							  <mrow>
								  \amp = \frac{(r+1)^4}{4}+C
							  </mrow>
						  </md>
					  </p>
				  

				  </solution>
			  </exercise>
			  
			  
			  <exercise>
				  <statement>
					  <p>
						  <m>\displaystyle \int x^2e^{2x} \, dx </m>
					  </p>
			  	
				  </statement>

			  
				  <solution>
					  <p>
						  Use integration by parts with 
						  <md>
							  <mrow>
								  u \amp = x^2 \amp dv \amp = e^{2x} \, dx
							  </mrow>
							  <mrow>
								  du \amp = 2x \, dx  \amp v \amp = \frac{1}{2} e^{2x}
							  </mrow>
						  </md>
						  Then
						  <md>
							  <mrow>
								  \int x^2e^{2x} \, dx \amp = x^2\cdot \frac{1}{2}e^{2x} - \int \frac{1}{2}e^{2x} \cdot 2x \, dx
							  </mrow>
							  <mrow>
								  \amp = \frac{1}{2}x^2 e^{2x} - \int xe^{2x} \, dx
							  </mrow>
						  </md>
						  We  now use integration by parts again on the new integral.
						  <md>
							  <mrow>
								  u \amp = x \amp dv \amp = e^{2x} \, dx
							  </mrow>
							  <mrow>
								  du \amp = dx \amp v \amp = \frac{1}{2} e^{2x}
							  </mrow>
						  </md>
						  So
						  <md>
							  <mrow>
							  	\int x^2e^{2x} \, dx \amp = \frac{1}{2}x^2 e^{2x} - \left( x\cdot \frac{1}{2} e^{2x} - \int \frac{1}{2} e^{2x} \, dx\right)
							  </mrow>
							  <mrow>
								  \amp = \frac{1}{2}x^2 e^{2x} - \frac{1}{2}xe^{2x} +\frac{1}{4}e^{2x} + C
							  </mrow>
						  </md>
					  </p>

				  </solution>
			  </exercise>
			  
			  
			  <exercise>
				  <statement>
					  <p>
						 <m>\displaystyle \int \frac{\cos(\sqrt{x})}{\sqrt{x}} \, dx </m>
					  </p>

				  </statement>

			  
				  <solution>
					  <p>
						  Use substitution with <m>u=\sqrt{x}=x^{1/2}</m> and <m>du = \dfrac{1}{2\sqrt{x}} \, dx</m>, so <m>2 \, du = \dfrac{1}{\sqrt{x}} \, dx</m>:
						  <md>
							  <mrow>
								  \int \frac{\cos(\sqrt{x})}{\sqrt{x}} \, dx \amp = \int 2 \cos(u) \, du
							  </mrow>
							  <mrow>
								  \amp = 2\sin(u) + C
							  </mrow>
							  <mrow>
								  \amp = 2\sin(\sqrt{x}) + C
							  </mrow>
						  </md>
					  </p>
				  
				  </solution>
			  </exercise>
			  
			  
			  <exercise>
				  <statement>
					  <p>
						 <m>\displaystyle \int \frac{7x}{(x-2)(x+3)} \, dx </m>
					  </p>

				  </statement>

			  
				  <solution>
					  <p>
						  First decompose the integrand into partial fractions:
						  <me>
							  \frac{7x}{(x-2)(x+3)} = \frac{A}{x-2} + \frac{B}{x+3}
						  </me>
						  This yields
						  <me>
							  7x = A(x+3) + B(x-2)
						  </me>.
						  Plug in <m>x=2</m> to solve for <m>A</m> and <m>x=-3</m> to solve for <m>B</m>:
						  <me>14 = 5A + 0 \implies A=\frac{14}{5}</me>
						  <me>-21 = 0 - 5B \implies B=\frac{21}{5}</me>
						  Now perform the integration:
						  <md>
							  <mrow>
								  \int \frac{7x}{(x-2)(x+3)} \, dx \amp = \int \left( \frac{14}{5} \cdot \frac{1}{x-2} + \frac{21}{5} \cdot \frac{1}{x+3}\right) \, dx
							  </mrow>
							  <mrow>
								  \amp = \frac{14}{5}\ln|x-2| + \frac{21}{5} \ln|x+3| + C
							  </mrow>
						  </md>
					  </p>
				  
				  </solution>
			  </exercise>
			  
			  
			  <exercise>
				  <statement>
					  <p>
						 <m>\displaystyle \int (e^x+3^x) \, dx </m>
					  </p>

				  </statement>
			  
				  <solution>
					  <p>
						  <md>
							  <mrow>
								  \int (e^x+3^x) \, dx \amp = e^x + \frac{1}{\ln(3)}\cdot 3^x +C
							  </mrow>
						  </md>
					  </p>
				  
				  </solution>
			  </exercise>
			  
			  
			  <exercise>
				  <statement>
					  <p>
						 <m>\displaystyle \int \frac{1}{x\ln(x)} \, dx </m>
					  </p>
				  </statement>

			  
				  <solution>
					  <p>
						  Use substitution with <m>u=\ln(x)</m> and <m>du=\dfrac{1}{x} \, dx</m>:
						  <md>
							  <mrow>
								  \int \frac{1}{x\ln(x)} \, dx \amp = \int \frac{1}{u} \, du
							  </mrow>
							  <mrow>
								  \amp = \ln|u| + C
							  </mrow>
							  <mrow>
								  \amp = \ln|\ln(x)|+C
							  </mrow>
						  </md>
					  </p>
				  
				  </solution>
			  </exercise>
			  
			  
			  
			  <exercise>
				  <statement>
					  <p>
						  <m>\displaystyle \int \sin^5(2\theta)\cos(2\theta) \, d\theta </m>
					  </p>

				  </statement>

			  
				  <solution>
					  <p>
						  Use substitution with <m>u=\sin(2\theta)</m> and <m>du = 2\cos(2\theta) \, d\theta</m>, so <m>\dfrac{1}{2} \, du = \cos(2\theta) \, d\theta</m>:
						  <md>
							  <mrow>
								  \int \sin^5(2\theta)\cos(2\theta) \, d\theta \amp = \int \frac{1}{2} u^5 \, du
							  </mrow>
							  <mrow>
								  \amp = \frac{1}{2} \frac{u^6}{6} + C
							  </mrow>
							  <mrow>
								  \amp = \frac{\sin^6(2\theta)}{12} + C
							  </mrow>
						  </md>
					  </p>
				  
				  </solution>
			  </exercise>
			  
			  
			  <exercise>
				  <statement>
					  <p>
						  <m>\displaystyle \int \frac{2x^2}{(9+x^3)^2} \, dx </m>
					  </p>
			  	
				  </statement>

			  
				  <solution>
					  <p>
						  Use substitution with <m>u=9+x^3</m> and <m>du = 3x^2 \, dx</m>, so <m>\dfrac{1}{3} \, du = x^2 \, dx</m>:
						  <md>
							  <mrow>
								  \int \frac{2x^2}{(9+x^3)^2} \, dx \amp = \int \frac{2}{3} u^{-2} \, du
							  </mrow>
							  <mrow>
								  \amp = \frac{2}{3}\frac{u^{-1}}{-1} + C
							  </mrow>
							  <mrow>
								  \amp = -\frac{2}{3}\cdot \frac{1}{9+x^3} + C
							  </mrow>
						  </md>
					  </p>
				  
				  </solution>
			  </exercise>
			 
			  
		  </exercises>
	  </section>
	  
	  
	  
	  
	  
	  
	  